\setcounter{section}{-1}
\section{Pr√°ctica 0}
\subsection{}
$\Sigma^0 = \{\lambda\}$

$\Sigma^1 = \Sigma = \{a, b\}$

$\Sigma^2 = \Sigma . \Sigma = \{aa, ab, ba, bb\}$

$\Sigma^* = \cup_{i \geq 0} \Sigma^i = \{\lambda, a, b, aa, bb, ab, bb, aaa, \ldots\}$

$\Sigma^+ = \cup_{i \geq 1} \Sigma^i = \{a, b, aa, bb, ab, bb, aaa, \ldots\}$

$|\Sigma| = 2$

$|\Sigma^0| = 1$

\subsection{}
$x^0 = \lambda$

$x^1 = abb$

$x^2 = abbabb$

$x^3 = abbabbabb$

$x^0.x^1.x^2.x^3 = abbabbabbabbabbabb$

$x^r = bba$

\subsection{}
\subsubsection{}
Falso

\subsubsection{}
Falso. $\lambda$ ni siquiera es un conjunto

\subsubsection{}
Falso

\subsubsection{}
Verdadero

\subsubsection{}
Verdadero

\subsubsection{}
Falso

\subsection{}
$xy = abbacb$

$(xy)^r = cbabba$

$y^r = cba$

$y^rx^r = cbabba$

$\lambda x = abb$

$\lambda y = abc$

$x \lambda y = abbabc$

$x^2 \lambda^3 y^2 = abbabbabcabc$

\subsection{}
$\Sigma \cup A = \{a,b,c\}$

$\Sigma \cap A = \{a\}$

$\Sigma . A = \{aa, ac, ba, bc\}$

$\Sigma . A^+ = \{aa, ba, ac, bc, aaa, baa, aca, bca, \ldots\}$

$\Sigma^+ . A = \{aa, ba, ac, bc, aaa, baa, aba, abc, \ldots\}$

$(\Sigma . A)^+ = \{aa, ac, ba, bc, aaaa, aaac, aaba, aabc, acaa, acac, acba, acbc, \ldots\}$

$(\Sigma . A)^* = \{\lambda, aa, ac, ba, bc, aaaa, aaac, aaba, aabc, acaa, acac, acba, acbc, \ldots\}$

$\Sigma^* . A^* = \{\lambda, aa, ac, ba, bc, aaa, aac, aba, abc, baa, bac, bba, bbc, aca, acc, bca, bcc, \ldots\}$

$\Sigma . \Lambda . A = \Sigma . A = \{aa, ac, ba, bc\}$

\subsection{}
\subsubsection{}
Verdadero

\subsubsection{}
Verdadero

\subsubsection{}
Verdadero

\subsubsection{}
Verdadero

\subsubsection{}
Falso

\subsubsection{}
Verdadero

\subsubsection{}
Verdadero

\subsubsection{}
Verdadero

\subsection{}
\subsubsection{}
a, b, $\lambda$, aa, ab

\subsubsection{}
a, b, aa, ab

\subsubsection{}
b, ab, bb, abb, aabb

\subsubsection{}
a, ab, aa, aab, aabb

\subsubsection{}
acbabbabbab, aacbabbabbab, aaaaacbabbabbab, aaaaacacbabbabbabbab

\subsubsection{}
$\lambda$, aaa, aba, abb, bab, baa, aaaaba, baaabb, bababa, bbbbbbb

\subsubsection{}
aa, bb, abba, bbbb, aaaa, baab

\subsubsection{}
a, b, aa, bb, aaaa, abba, baab, bbbb

\subsection{}
$L_1 = \{a^kb^k | k \geq 1\}$

$L_2 = \{a^{2k}b^k | k \geq 1\}$

$L_3 = \{a^kbc^k | k \geq 3\}$

\subsection{}
\subsubsection{}
$|a . (a . \alpha) = 1 + |a . \alpha| = 2 + |\alpha|$

\subsection{}
\subsubsection{}
Quiero ver que $\forall \alpha (\alpha \in F(F(A)) \Leftrightarrow \alpha \in F(A))$

\begin{tabular}{l l}
    $\alpha \in F(F(A))$ & $ \Leftrightarrow \exists \beta (\beta \alpha \in F(A)) $ \\
                         & $ \Leftrightarrow \exists \beta \exists \gamma (\gamma \beta \alpha \in A) $ \\
                         & $ \Leftrightarrow \exists \phi (\phi \in A)$ tal que $\phi = \gamma \beta $ \\
\end{tabular}

\subsubsection{}
Quiero ver que $\forall \alpha (\alpha \in F(F(A)) \Leftrightarrow \alpha \in F(A))$

\begin{tabular}{l l}
    $\alpha \in S(S(A))$ & $ \Leftrightarrow \exists \beta (\alpha \beta \in S(A)) $ \\
                         & $ \Leftrightarrow \exists \beta \exists \gamma (\alpha \beta \gamma \in A) $ \\
                         & $ \Leftrightarrow \exists \phi (\phi \alpha \in A)$ tal que $\phi = \gamma \beta $ \\
\end{tabular}

\subsubsection{}
Quiero ver que $\forall \alpha (\alpha \in F(AB) \Leftrightarrow \alpha \in F(B) \lor \alpha \in F(A)B)$

$\Rightarrow )$

\begin{tabular}{l l}
    $\alpha \in F(AB)$ & $\Rightarrow \exists w (w \alpha \in AB)$ \\
                       & $\Rightarrow wxyz \in AB $ con $xyz = \alpha$ \\
                       & $\Rightarrow (w \in A \land xyz \in B) \lor (wx \in A \land yz \in B) \lor (wxy \in A \land z \in B)$ \\
                       & $\Rightarrow (xyz \in B) \lor (x \in F(A) \land yz \in B) \lor (xy \in (F(A) \land z \in B))$ \\
                       & $\Rightarrow (xyz \in B) \lor (xyz \in F(A)B) \lor (xyz \in F(A)B)$ \\
                       & $\Rightarrow (xyz \in B) \lor (xyz \in F(A)B)$ \\
                       & $\Rightarrow (\alpha \in B) \lor (\alpha \in F(A)B)$ \\
                       & $\Rightarrow (\alpha \in F(B) \lor (\alpha \in F(A)B)$ \\
\end{tabular}

$\Leftarrow )$

\begin{tabular}{l l}
    $\alpha \in F(B)$ & $\Rightarrow \exists \beta (\beta \alpha \in B)$ \\
                      & $\Rightarrow \exists \gamma (\gamma \beta \alpha \in AB)$ con $\gamma \in A$ \\
                      & $\Rightarrow \alpha \in F(AB)$ \\

    $\alpha \in F(A)B$ & $\Rightarrow$ reemplazando $\alpha$ por $yz$, $yz \in F(A)B$ con $y \in F(A), z \in B$ \\
                       & $\Rightarrow \exists x (xy \in A)$ \\
                       & $\Rightarrow xyz \in AB$ \\
                       & $\Rightarrow x \alpha \in AB$ \\
                       & $\Rightarrow \alpha \in F(AB)$ \\
\end{tabular}
